seiostar/LogRelSourceTarget.CompatibilityLemmas.fst
@@ -8,9 +8,9 @@ open LambdaIO
 open LambdaIO.ConstructLemmas
 open IOStar
 open IOStar.DestructLemmas
-open QTypes.EvalEnv
 open QTypes.Subst
 open QTypes.Sem
+open QTypes.HelperTactics
 open LogRelSourceTarget
 
 let bind_squash (a #b:Type) (f:a -> GTot (squash b)) : Pure (squash b) (requires a) (ensures fun _ -> True) = 
@@ -118,7 +118,7 @@ let compat_oval_var g (x:var{Some? (g x)}) : Lemma (fs_oval_var g x ⊏ EVar x) 
 let compat_oval_var0 (g:typ_env) (t:qType) : Lemma (fs_oval_var0 g t ⊏ EVar 0) =
   introduce forall b (s:gsub (extend t g) b) fsG h. fsG `(≍) h` s ==>  t ⊆ (h, hd fsG, gsubst s (EVar 0)) with begin
     introduce _ ==> _ with _. begin
-      index_0_hd fsG;
+      lem_index_0_hd fsG;
       assert (t ∈ (h, hd fsG, s 0));
       lem_values_are_expressions t h (hd fsG) (s 0)
     end
@@ -1153,7 +1153,7 @@ let compat_oprod_if #g
       let fs_e = fs_prod_bind fs_e1' (fun x -> fs_prod_if_val x fs_e2' fs_e3') in
       assert (fs_e == fs_oprod_if fs_e1 fs_e2 fs_e3 fsG) by (
         norm [delta_only [`%fs_oprod_if;`%fs_oprod_bind';`%fs_oprod_bind;`%fs_oprod_if_val]];
-        l_to_r [`lem_hd_stack;`tail_stack_inverse];
+        simplify_stack_ops ();
         trefl ());
       let e = EIf (gsubst s e1) (gsubst s e2) (gsubst s e3) in
       assert (gsubst s (EIf e1 e2 e3) == e);
@@ -1245,7 +1245,7 @@ let compat_oprod_app #g (#a #b:qType) (fs_f:fs_oprod g (a ^->!@ b)) (fs_x:fs_opr
       let fs_e = fs_prod_bind fs_f' (fun f' -> fs_prod_bind fs_x' (fun x' -> f' x')) in
       assert (fs_e == fs_oprod_app fs_f fs_x fsG) by (
         norm [delta_only [`%fs_oprod_app;`%fs_oprod_bind';`%fs_oprod_bind;`%fs_oprod_app_oval_oval]];
-        l_to_r [`lem_hd_stack;`tail_stack_inverse];
+        simplify_stack_ops ();
         trefl ());
       let e = EApp (gsubst s f) (gsubst s x) in
       assert (gsubst s (EApp f x) == e);
@@ -1741,7 +1741,7 @@ let compat_oprod_pair #g
       let fs_e = fs_prod_bind fs_e1' (fun v1 -> fs_prod_bind #t2 #(t1 ^* t2) fs_e2' (fun v2 -> return (v1, v2))) in
       assert (fs_e == fs_oprod_pair fs_e1 fs_e2 fsG) by (
         norm [delta_only [`%fs_oprod_pair;`%fs_oprod_bind';`%fs_oprod_bind;`%fs_oprod_return_val;`%fs_val_pair]];
-        l_to_r [`lem_hd_stack;`tail_stack_inverse];
+        simplify_stack_ops ();
         trefl ());
       let e = EPair (gsubst s e1) (gsubst s e2) in
       assert (gsubst s (EPair e1 e2) == e);
@@ -1838,7 +1838,7 @@ let compat_oprod_string_eq #g
       let fs_e = fs_prod_bind fs_e1' (fun v1 -> fs_prod_bind #qString #qBool fs_e2' (fun v2 -> return (v1 = v2))) in
       assert (fs_e == fs_oprod_string_eq fs_e1 fs_e2 fsG) by (
         norm [delta_only [`%fs_oprod_string_eq;`%fs_oprod_bind';`%fs_oprod_bind;`%fs_oprod_return_val]];
-        l_to_r [`lem_hd_stack;`tail_stack_inverse];
+        simplify_stack_ops ();
         trefl ());
       let e = EStringEq (gsubst s e1) (gsubst s e2) in
       assert (gsubst s (EStringEq e1 e2) == e);
@@ -1871,7 +1871,7 @@ let compat_oprod_fst #g
       let fs_e = fs_prod_bind #(t1 ^* t2) #t1 fs_e12' (fun v -> return (fst #(fs_val t1) #(fs_val t2) v)) in
       assert (fs_e == (fs_oprod_fmap #g #(t1 ^* t2) #t1 fs_e12 fst) fsG) by (
         norm [delta_only [`%fs_oprod_fmap;`%fs_oprod_bind';`%fs_oprod_bind;`%fs_oprod_return_val]];
-        l_to_r [`lem_hd_stack;`tail_stack_inverse];
+        simplify_stack_ops ();
         trefl ());
       let e = EFst (gsubst s e12) in
       assert (gsubst s (EFst e12) == e);
@@ -1900,7 +1900,7 @@ let compat_oprod_snd #g (#t1 #t2:qType) (fs_e12:fs_oprod g (t1 ^* t2)) (e12:exp)
       let fs_e = fs_prod_bind #(t1 ^* t2) #t2 fs_e12' (fun v -> return (snd #(fs_val t1) #(fs_val t2) v)) in
       assert (fs_e == (fs_oprod_fmap #g #(t1 ^* t2) #t2 fs_e12 snd) fsG) by (
         norm [delta_only [`%fs_oprod_fmap;`%fs_oprod_bind';`%fs_oprod_bind;`%fs_oprod_return_val]];
-        l_to_r [`lem_hd_stack;`tail_stack_inverse];
+        simplify_stack_ops ();
         trefl ());
       let e = ESnd (gsubst s e12) in
       assert (gsubst s (ESnd e12) == e);
@@ -1939,7 +1939,7 @@ let compat_oprod_case #g (#a #b #c:qType)
       let fs_e = fs_prod_bind fs_sc (fun x -> fs_prod_case_val x fs_il fs_ir) in
       assert (fs_e == fs_oprod_case fs_cond fs_inlc fs_inrc fsG) by (
         norm [delta_only [`%fs_oprod_case;`%fs_prod_case_val;`%fs_oprod_bind';`%fs_oprod_bind;`%fs_oprod_case_val]];
-        l_to_r [`lem_hd_stack;`tail_stack_inverse];
+        simplify_stack_ops ();
         trefl ());
       let e = ECase (gsubst s cond) (subst (sub_elam s) inlc) (subst (sub_elam s) inrc) in
       assert (gsubst s (ECase cond inlc inrc) == e);
@@ -1969,7 +1969,7 @@ let compat_oprod_inl #g (t1 t2:qType) (fs_e:fs_oprod g t1) (e:exp)
       let fs_ex = fs_prod_bind #t1 #(t1 ^+ t2) fs_e' (fun v -> return (Inl #(fs_val t1) #(fs_val t2) v)) in
       assert (fs_ex == (fs_oprod_fmap #g #t1 #(t1 ^+ t2) fs_e Inl) fsG) by (
         norm [delta_only [`%fs_oprod_fmap;`%fs_oprod_bind';`%fs_oprod_bind;`%fs_oprod_return_val]];
-        l_to_r [`lem_hd_stack;`tail_stack_inverse];
+        simplify_stack_ops ();
         trefl ());
       let ex = EInl (gsubst s e) in
       assert (gsubst s (EInl e) == ex);
@@ -1999,7 +1999,7 @@ let compat_oprod_inr #g (t1 t2:qType) (fs_e:fs_oprod g t2) (e:exp)
       let fs_ex = fs_prod_bind #t2 #(t1 ^+ t2) fs_e' (fun v -> return (Inr #(fs_val t1) #(fs_val t2) v)) in
       assert (fs_ex == (fs_oprod_fmap #g #t2 #(t1 ^+ t2) fs_e Inr) fsG) by (
         norm [delta_only [`%fs_oprod_fmap;`%fs_oprod_bind';`%fs_oprod_bind;`%fs_oprod_return_val]];
-        l_to_r [`lem_hd_stack;`tail_stack_inverse];
+        simplify_stack_ops ();
         trefl ());
       let ex = EInr (gsubst s e) in
       assert (gsubst s (EInr e) == ex);
@@ -2029,7 +2029,7 @@ let compat_oprod_openfile #g (fs_fnm:fs_oprod g qString) (fnm:exp)
       let fs_e = fs_prod_bind fs_fnm' (fun fnm' -> io_call OOpen fnm') in
       assert (fs_e == (fs_oprod_call OOpen fs_fnm) fsG) by (
         norm [delta_only [`%fs_oprod_call;`%fs_oprod_bind';`%fs_oprod_bind;`%fs_oprod_return]];
-        l_to_r [`lem_hd_stack;`tail_stack_inverse];
+        simplify_stack_ops ();
         trefl ());
       let e = EOpen (gsubst s fnm) in
       assert (gsubst s (EOpen fnm) == e);
@@ -2059,7 +2059,7 @@ let compat_oprod_read #g (fs_fd:fs_oprod g qFileDescr) (fd:exp)
       let fs_e = fs_prod_bind fs_fd' (fun fd' -> io_call ORead fd') in
       assert (fs_e == (fs_oprod_call ORead fs_fd) fsG) by (
         norm [delta_only [`%fs_oprod_call;`%fs_oprod_bind';`%fs_oprod_bind;`%fs_oprod_return]];
-        l_to_r [`lem_hd_stack;`tail_stack_inverse];
+        simplify_stack_ops ();
         trefl ());
       let e = ERead (gsubst s fd) in
       assert (gsubst s (ERead fd) == e);
@@ -2091,7 +2091,7 @@ let compat_oprod_write #g (fs_fd:fs_oprod g qFileDescr) (fs_msg:fs_oprod g qStri
       let fs_e = fs_prod_bind fs_pair' (fun args' -> io_call OWrite args') in
       assert (fs_e == (fs_oprod_call OWrite (fs_oprod_pair fs_fd fs_msg)) fsG) by (
         norm [delta_only [`%fs_oprod_call;`%fs_oprod_pair;`%fs_oprod_bind';`%fs_oprod_bind;`%fs_oprod_return;`%fs_oprod_return_val;`%fs_val_pair;`%fs_prod_bind]];
-        l_to_r [`lem_hd_stack;`tail_stack_inverse];
+        simplify_stack_ops ();
         trefl ());
       let e = EWrite (gsubst s fd) (gsubst s msg) in
       assert (gsubst s (EWrite fd msg) == e);
@@ -2121,7 +2121,7 @@ let compat_oprod_close #g (fs_fd:fs_oprod g qFileDescr) (fd:exp)
       let fs_e = fs_prod_bind fs_fd' (fun fd' -> io_call OClose fd') in
       assert (fs_e == (fs_oprod_call OClose fs_fd) fsG) by (
         norm [delta_only [`%fs_oprod_call;`%fs_oprod_bind';`%fs_oprod_bind;`%fs_oprod_return]];
-        l_to_r [`lem_hd_stack;`tail_stack_inverse];
+        simplify_stack_ops ();
         trefl ());
       let e = EClose (gsubst s fd) in
       assert (gsubst s (EClose fd) == e);
